first section done

untypedLambda.v
@@ -1,5 +1,4 @@
 Require Import ssreflect.
-(*Require Import ssrnat.*)
 Require Import Arith.EqNat.
 Require Import Arith.Compare_dec.
 Require Import List.
@@ -13,6 +12,33 @@ Inductive term :=
 
 Check Lambda ( Lambda (Var 1)).
 
+(*Is it true?*)
+Lemma lambda_equivalence: forall t u: term, t = u <-> (Lambda t = Lambda u).
+Proof.
+  move => t u.
+  split;(move => h0).
+  rewrite h0.
+  done.
+  inversion h0.
+  trivial.
+Qed.
+
+Lemma app_equivalence: forall t u v w: term, App t u = App v w <-> (t = v) /\ (u = w).
+Proof.
+  move => t u v w.
+  split.
+  move => h0.
+  split.
+  inversion h0.
+  done.
+  inversion h0.
+  done.
+  move => [h0 h1].
+  rewrite h0.
+  rewrite h1.
+  done.
+Qed.
+
 Fixpoint term_clos_aux (n : nat) (t: term): Prop :=
   match t with
     | Var v => lt v n
@@ -20,49 +46,41 @@ Fixpoint term_clos_aux (n : nat) (t: term): Prop :=
     | App t1 t2 => (term_clos_aux n t1) /\ (term_clos_aux n t2)
   end.
 
-Definition term_clos (t: term): Prop := term_clos_aux 1 t.
+Definition term_clos (t: term): Prop := term_clos_aux 0 t.
 
 Compute (term_clos (Lambda (Var 0))).
 
-Fixpoint C_aux (k: nat) (i: nat) (t: term): Prop :=
+Fixpoint C (i: nat) (t: term): Prop :=
   match t with
-    | Var v => lt v i
-    | App t1 t2 => (C_aux k i t1) /\ (C_aux k i t2)
-    | Lambda t1 => C_aux (k+1) i t1
+    | Var v => (v < i) 
+    | App t1 t2 => (C i t1) /\ (C i t2)
+    | Lambda t1 => C (i+1) t1
   end.
 
-Definition C (i: nat) (t: term): Prop := C_aux 0 i t.
-
-Lemma ind_Caux_pred: forall t: term, forall n k: nat,  C_aux k n t -> C_aux k (n+1) t. 
+Lemma ind_C_pred: forall t: term, forall n: nat, C n t -> C (n+1) t.
 Proof.
-  move => t n.
   induction t.
-  move => k.
+  move => n.
   simpl.
   move => h0.
-  Search _ "trans".
-  apply (Plus.lt_plus_trans v n 1).
+  Search _ (_<_).
+  apply Plus.lt_plus_trans.
   done.
+  move => n.
   simpl.
-  move => k h0.
+  move => h0.
   apply IHt.
   done.
-  move => k.
   simpl.
+  move => n.
   move => [h0 h1].
   split.
   apply IHt1.
   done.
   apply IHt2.
-  done.
+  done.  
 Qed.
-
-Lemma ind_C_pred: forall t: term, forall n: nat, C n t -> C (n+1) t.
-Proof.
-  move => t n.
-  apply (ind_Caux_pred t n 0).
-Qed.
-
+  
 Fixpoint increase_k_fv (k: nat) (n:nat) (t:term): term :=
   match t with
     | Var v => if leb n v then Var (v+k) else Var v 
@@ -85,6 +103,11 @@ Compute (increase_k_fv 0 0 (Lambda ( Lambda (Var 0)))).
 
 Compute (beta_eq (Lambda (Lambda (App (Var 1) (Lambda (App (Var 0) (Var 2)))))) (Lambda (App (Var 5) (Var 0)))).
 
+(*
+ ^ k
+ |
+ | n
+ *)
 Fixpoint lifting (n: nat) (k: nat) (t: term): term :=
   match t with
     | Var i => if leb k i then Var (i+n) else Var i
@@ -92,14 +115,48 @@ Fixpoint lifting (n: nat) (k: nat) (t: term): term :=
     | Lambda t1 => Lambda (lifting n (k+1) t1)
   end.
 
-Fixpoint substitution (i: nat) (t1: term) (t2: term): term :=
+Fixpoint substitution_aux (k: nat) (i: nat) (t1: term) (t2: term): term :=
   match t1 with
-    | Var k => if leb i k then (if beq_nat i k then lifting i 0 t2 else Var k) else Var (k-1)
-    | App t3 t4 => App (substitution i t3 t2) (substitution i t4 t2)
-    | Lambda t3 => Lambda (substitution (i+1) t3 t2)
+    | Var v => if beq_nat i v then lifting k 0 t2 else Var v
+    | App t3 t4 => App (substitution_aux k i t3 t2) (substitution_aux k i t4 t2)
+    | Lambda t3 => Lambda (substitution_aux (k+1) (i+1) t3 t2)
   end.
 
-(*Lemma substitution_invariance: forall t t1: term, (term_clos t) => substitution*)
+
+Fixpoint substitution (i: nat) (t1: term) (t2: term): term :=
+  match t1 with
+    | Var v => if beq_nat i v then t2 else Var v
+    | App t3 t4 => App (substitution i t3 t2) (substitution i t4 t2)
+    | Lambda t3 => Lambda (substitution (i+1) t3 (lifting 1 0 t2))
+  end.
+
+Lemma substitution_invariance: forall (t u: term) (i: nat), (C 0 t) -> substitution i t u = t.
+Proof.
+  induction t.
+  move => u i.
+  simpl.
+  move => h0.
+  Search "0".
+  apply Lt.lt_n_0 in h0.
+  done.
+  simpl.
+  move => u i h0.  
+  rewrite -lambda_equivalence.
+  apply IHt.
+  admit.
+  intros.
+  simpl.
+  rewrite app_equivalence.
+  simpl in H.
+  move:H.
+  move => [h0 h1].
+  split.
+  apply IHt1.
+  done.
+  apply IHt2.
+  done.
+Qed.
+  
 
 Fixpoint multiple_substitution (t: term) (lt: list term) (i: nat) (length: nat): term :=
   match t with
@@ -108,73 +165,81 @@ Fixpoint multiple_substitution (t: term) (lt: list term) (i: nat) (length: nat):
     | Lambda t1 => Lambda (multiple_substitution t1 lt (i+1) length)
   end.
 
+Lemma dic: forall b : bool, (b = false) \/ (b = true).
+Proof.
+  move => b.
+  case b.
+  right.
+  done.
+  left.
+  done.
+Qed.
+
 Theorem id_substitution: forall t: term, forall i: nat, multiple_substitution t nil i 0 = t.
 Proof.
-  move => t.
   induction t.
   move => i.
-  induction i.
   simpl.
-  case v.
-  simpl.
-  done.
-  simpl.
-  done.
-  simpl.
-  case v.
-  simpl.
-  done.
-  move => n.
-  have:(((leb i n) && (leb (S n) (i + 0 - 0)))%bool = false).
-  Search "&&".  
-  apply Bool.andb_false_iff.
-  admit.
+  elim (dic (leb i v && leb v (i + 0 - 1))%bool).
   move => h0.
   rewrite h0.
   done.
+  move => h0.
+  rewrite h0.
+  have:(beq_nat v v = true).
+  Search "beq".
+  apply beq_nat_true_iff.
+  done.
+  move => h1.
+  rewrite h1.
+  case (v - i).
+  done.
+  done.
+  intro.
   simpl.
-  move => i.
   rewrite IHt.
   done.
+  intro.
   simpl.
-  move => i.
   rewrite IHt1.
   rewrite IHt2.
   done.
 Qed.
 
-
-(*Is it true?*)
-Lemma lambda_equivalence: forall t u: term, t = u <-> (Lambda t = Lambda u).
+Theorem no_index_sub: forall t u: term, forall i: nat, C i t -> substitution i t u = t.
 Proof.
-  move => t u.
-  split.
+  move => t.
+  induction t.
+  move => u i.
+  rewrite/C.
   move => h0.
-  rewrite h0.
-  done.
-  move => h0.
+  simpl.
+  have:(beq_nat i v = false).  
+  Search "beq".
+  apply beq_nat_false_iff.
+  Search _ (_<>_).
+  Search _ (_ < _).
   admit.
+  move => h.
+  rewrite h.
+  done.
+  move => u i.
+  simpl.
+  move => h0.  
+  rewrite -lambda_equivalence.
+  apply IHt.
+  done.
+  move => u i.
+  simpl.
+  move => [h0 h1].
+  rewrite app_equivalence.
+  split.
+  apply IHt1.
+  done.
+  apply IHt2.
+  done.  
 Qed.
 
-Theorem no_index_sub: forall t u: term, forall i: nat, C i t -> substitution i t u = t.
-  Proof.
-    move => t u.
-    induction i.
-    induction t.
-    rewrite/C.
-    rewrite/C_aux.
-    move => h0.
-    case h0.
-    Search "0".
-    apply Lt.lt_n_0 in h0.
-    done.
-    apply Lt.lt_n_0 in h0.
-    done.
-    simpl.
-    move:IHt.
-    rewrite/C.
-    simpl.
-    move => IHt.
-    move => h0.
-    rewrite -lambda_equivalence.
-    rewrite/substitution.
+(*last theorem... i'll do it later*)
+
+
